src/lib/data/Kuiper.Tensor.fsti
@@ -518,11 +518,11 @@ fn tensor_apply_bij
   (f : abs d1 =~ abs d2)
   (#l : tlayout d1) {| is_full l |}
   (a : tensor et l)
-  (m : Chest.t d1 et)
+  (#fp : perm) (#m : Chest.t d1 et)
   requires
-    a |-> m
+    a |-> Frac fp m
   ensures
-    from_array (tlayout_bij f l) (core a) |-> Chest.mk d2 (fun i -> Chest.acc m (i <~| f))
+    from_array (tlayout_bij f l) (core a) |-> Frac fp (Chest.mk d2 (fun i -> Chest.acc m (i <~| f)))
 
 let unfold_index (#r: nat {r > 1}) (#d: idesc r) (i : abs (fold_outer d)): GTot (abs d) = 
   let ICons h1 (ICons h2 ts) = d in
